mqhasm/mQhasm.v
@@ -34,6 +34,8 @@ Module MakeQhasm (V : SsrOrderedType).
   Module VS := FSetList.Make V.
   Module VSLemmas := FSetLemmas VS.
 
+
+
   (** Syntax *)
 
   Definition var : Type := V.t.
@@ -82,11 +84,13 @@ Module MakeQhasm (V : SsrOrderedType).
     | hd::tl => VS.union (vars_instr hd) (vars_program tl)
     end.
 
+
+
   (** State *)
 
   Notation value := Z.
 
-  Module Store := MakePStore V.
+  Module Store := MakeTStore V.
 
   Module State.
 
@@ -94,19 +98,19 @@ Module MakeQhasm (V : SsrOrderedType).
 
     Definition empty : t := Store.empty value.
 
-    Definition acc (x : var) (s : t) : option value :=
+    Definition acc (x : var) (s : t) : value :=
       Store.acc x s.
 
     Definition upd (x : var) (v : value) (s : t) : t :=
       Store.upd x v s.
 
-    Definition unset (x : var) (s : t) : t :=
-      Store.unset x s.
+    Definition upd2 x1 v1 x2 v2 (s : t) : t :=
+      Store.upd x2 v2 (Store.upd x1 v1 s).
 
     Lemma acc_upd_eq :
       forall x y v (s : t),
         x == y ->
-        acc x (upd y v s) = Some v.
+        acc x (upd y v s) = v.
     Proof.
       exact: Store.acc_upd_eq.
     Qed.
@@ -119,44 +123,43 @@ Module MakeQhasm (V : SsrOrderedType).
       exact: Store.acc_upd_neq.
     Qed.
 
-    Lemma acc_empty :
-      forall x, acc x empty = None.
+    Lemma acc_upd2_eq1 :
+      forall x y1 v1 y2 v2 (s : t),
+        x == y1 ->
+        x != y2 ->
+        acc x (upd2 y1 v1 y2 v2 s) = v1.
     Proof.
-      exact: Store.acc_empty.
+      move=> x y1 v1 y2 v2 s Hx1 Hx2.
+      rewrite /upd2 (acc_upd_neq _ _ Hx2) (acc_upd_eq _ _ Hx1).
+      reflexivity.
     Qed.
 
-    Lemma acc_unset_eq :
-      forall x y s,
-        x == y ->
-        acc x (unset y s) = None.
+    Lemma acc_upd2_eq2 :
+      forall x y1 v1 y2 v2 (s : t),
+        x == y2 ->
+        acc x (upd2 y1 v1 y2 v2 s) = v2.
     Proof.
-      exact: Store.acc_unset_eq.
+      move=> x y1 v1 y2 v2 s Hx2.
+      rewrite /upd2 (acc_upd_eq _ _ Hx2).
+      reflexivity.
     Qed.
 
-    Lemma acc_unset_neq :
-      forall x y s,
-        x != y ->
-        acc x (unset y s) = acc x s.
+    Lemma acc_upd2_neq :
+      forall x y1 v1 y2 v2 s,
+        x != y1 ->
+        x != y2 ->
+        acc x (upd2 y1 v1 y2 v2 s) = acc x s.
     Proof.
-      exact: Store.acc_unset_neq.
+      move=> x y1 v1 y2 v2 s Hx1 Hx2.
+      rewrite /upd2 (acc_upd_neq _ _ Hx2) (acc_upd_neq _ _ Hx1).
+      reflexivity.
     Qed.
-
-    Definition Empty (s : t) : Prop := Store.Empty s.
 
     Definition Upd x v (s1 s2 : t) : Prop :=
       forall y, acc y s2 = acc y (upd x v s1).
 
     Definition Upd2 x1 v1 x2 v2 (s1 s2 : t) : Prop :=
       forall y, acc y s2 = acc y (upd x2 v2 (upd x1 v1 s1)).
-
-    Definition Unset x (s1 s2 : t) : Prop :=
-      forall y, acc y s2 = acc y (unset x s1).
-
-    Lemma Empty_acc :
-      forall x s, Empty s -> acc x s = None.
-    Proof.
-      exact: Store.Empty_acc.
-    Qed.
 
     Lemma Upd_upd :
       forall x v s,
@@ -173,18 +176,11 @@ Module MakeQhasm (V : SsrOrderedType).
       reflexivity.
     Qed.
 
-    Lemma Unset_unset :
-      forall x s,
-        Unset x s (unset x s).
-    Proof.
-      exact: Store.Unset_unset.
-    Qed.
-
     Lemma acc_Upd_eq :
       forall x y v s1 s2,
         x == y ->
         Upd y v s1 s2 ->
-        acc x s2 = Some v.
+        acc x s2 = v.
     Proof.
       exact: Store.acc_Upd_eq.
     Qed.
@@ -203,23 +199,22 @@ Module MakeQhasm (V : SsrOrderedType).
         x == y1 ->
         x != y2 ->
         Upd2 y1 v1 y2 v2 s1 s2 ->
-        acc x s2 = Some v1.
+        acc x s2 = v1.
     Proof.
       move=> x y1 v1 y2 v2 s1 s2 Heq Hne Hupd.
       rewrite (Hupd x).
-      rewrite (acc_upd_neq _ _ Hne).
-      rewrite (acc_upd_eq _ _ Heq).
-      reflexivity.
+      exact: acc_upd2_eq1.
     Qed.
 
     Lemma acc_Upd2_eq2 :
       forall x y1 v1 y2 v2 s1 s2,
         x == y2 ->
         Upd2 y1 v1 y2 v2 s1 s2 ->
-        acc x s2 = Some v2.
+        acc x s2 = v2.
     Proof.
       move=> x y1 v1 y2 v2 s1 s2 Heq Hupd.
-      exact: (acc_Upd_eq Heq Hupd).
+      rewrite (Hupd x).
+      exact: acc_upd2_eq2.
     Qed.
 
     Lemma acc_Upd2_neq :
@@ -231,30 +226,12 @@ Module MakeQhasm (V : SsrOrderedType).
     Proof.
       move=> x y1 v1 y2 v2 s1 s2 Hne1 Hne2 Hupd.
       rewrite (Hupd x).
-      rewrite (acc_upd_neq _ _ Hne2).
-      rewrite (acc_upd_neq _ _ Hne1).
-      reflexivity.
-    Qed.
-
-    Lemma acc_Unset_eq :
-      forall x y s1 s2,
-        x == y ->
-        Unset y s1 s2 ->
-        acc x s2 = None.
-    Proof.
-      exact: Store.acc_Unset_eq.
-    Qed.
-
-    Lemma acc_Unset_neq :
-      forall x y s1 s2,
-        x != y ->
-        Unset y s1 s2 ->
-        acc x s2 = acc x s1.
-    Proof.
-      exact: Store.acc_Unset_neq.
+      exact: acc_upd2_neq.
     Qed.
 
   End State.
+
+
 
   (** Semantics *)
 
@@ -270,204 +247,81 @@ Module MakeQhasm (V : SsrOrderedType).
     | QMul => (v1 * v2)%Z
     end.
 
-  Inductive eval_exp : exp -> value -> State.t -> Prop :=
-  | EQVar :
-      forall v n s,
-        State.acc v s = Some n ->
-        eval_exp (QVar v) n s
-  | EQConst : forall n s, eval_exp (QConst n) n s
-  | EQUnop :
-      forall op e n m s,
-        eval_exp e n s ->
-        eval_unop op n = m ->
-        eval_exp (QUnop op e) m s
-  | EQBinop :
-      forall op e1 e2 v1 v2 n s,
-        eval_exp e1 v1 s ->
-        eval_exp e2 v2 s ->
-        eval_binop op v1 v2 = n ->
-        eval_exp (QBinop op e1 e2) n s
-  | EQPow :
-      forall e n m s,
-        eval_exp e m s ->
-        eval_exp (QPow e n) (m^(Zpos n)) s.
+  Fixpoint eval_exp (e : exp) (s : State.t) : value :=
+    match e with
+    | QVar v => State.acc v s
+    | QConst n => n
+    | QUnop op e => eval_unop op (eval_exp e s)
+    | QBinop op e1 e2 => eval_binop op (eval_exp e1 s) (eval_exp e2 s)
+    | QPow e p => (eval_exp e s) ^ (Zpos p)
+    end.
 
-  Inductive eval_instr : State.t -> instr -> State.t -> Prop :=
-  | EQAssign :
-      forall v e n s1 s2,
-        eval_exp e n s1 ->
-        State.Upd v n s1 s2 ->
-        eval_instr s1 (QAssign v e) s2
-  | EQSplit :
-      forall v1 v2 e i n1 n2 n s1 s2,
-        eval_exp e n s1 ->
-        State.Upd2 v1 n1 v2 n2 s1 s2 ->
-        n1 = fst (Z.div_eucl n (2^(Zpos i))) ->
-        n2 = snd (Z.div_eucl n (2^(Zpos i))) ->
-        eval_instr s1 (QSplit v1 v2 e i) s2.
+  Definition eval_instr (s : State.t) (i : instr) : State.t :=
+    match i with
+    | QAssign v e => State.upd v (eval_exp e s) s
+    | QSplit vh vl e i =>
+      let (q, r) := Z.div_eucl (eval_exp e s) (2^(Zpos i)) in
+      State.upd2 vh q vl r s
+    end.
 
-  Inductive eval_program : State.t -> program -> State.t -> Prop :=
-  | EQEmpty : forall s, eval_program s nil s
-  | EQCons :
-      forall hd tl s1 s2 s3,
-        eval_instr s1 hd s2 ->
-        eval_program s2 tl s3 ->
-        eval_program s1 (hd::tl) s3.
-
-  Lemma eval_qvar_unique v n m s :
-    let e := QVar v in
-    eval_exp e n s -> eval_exp e m s -> n == m.
-  Proof.
-    move=> e Hn Hm.
-    inversion_clear Hn.
-    inversion_clear Hm.
-    move: H H0; case: (State.acc v s).
-    + move=> u [] Hun [] Hum.
-      rewrite -Hun -Hum; exact: eqxx.
-    + discriminate.
-  Qed.
-
-  Lemma eval_qconst_unique v n m s :
-    let e := QConst v in
-    eval_exp e n s -> eval_exp e m s -> n == m.
-  Proof.
-    move=> e Hn Hm.
-    have: (v = n /\ v = m).
-    - split.
-      + inversion_clear Hn.
-        reflexivity.
-      + inversion_clear Hm.
-        reflexivity.
-    - move=> [] Hvn Hvm; rewrite -Hvn -Hvm; exact: eqxx.
-  Qed.
-
-  Lemma eval_qunop_unique :
-    forall (op : unop) (e : exp),
-      (forall (n m : value) (s : State.t),
-          eval_exp e n s -> eval_exp e m s -> n == m) ->
-      forall (n m : value) (s : State.t),
-        eval_exp (QUnop op e) n s ->
-        eval_exp (QUnop op e) m s ->
-        n == m.
-  Proof.
-    move=> op e Hind n m s Hn Hm.
-    inversion_clear Hn.
-    inversion_clear Hm.
-    move: (Hind _ _ _ H H1) => {H H1} H01.
-    rewrite -H0 -H2 (eqP H01).
-    exact: eqxx.
-  Qed.
-
-  Lemma eval_qbinop_unique :
-    forall (op : binop) (e1 : exp),
-      (forall (n m : value) (s : State.t),
-          eval_exp e1 n s -> eval_exp e1 m s -> n == m) ->
-      forall e2 : exp,
-        (forall (n m : value) (s : State.t),
-            eval_exp e2 n s -> eval_exp e2 m s -> n == m) ->
-        forall (n m : value) (s : State.t),
-          eval_exp (QBinop op e1 e2) n s ->
-          eval_exp (QBinop op e1 e2) m s ->
-          n == m.
-  Proof.
-    move=> op e1 Hind1 e2 Hind2 n m s Hn Hm.
-    inversion_clear Hn.
-    inversion_clear Hm.
-    move: (Hind1 _ _ _ H H2) => {H H2} => H10.
-    move: (Hind2 _ _ _ H0 H3) => {H0 H3} => H23.
-    rewrite -H1 -H4 (eqP H10) (eqP H23).
-    exact: eqxx.
-  Qed.
-
-  Lemma eval_qpow_unique :
-    forall e : exp,
-      (forall (n m : value) (s : State.t),
-          eval_exp e n s -> eval_exp e m s -> n == m) ->
-      forall (p : positive) (n m : value) (s : State.t),
-        eval_exp (QPow e p) n s ->
-        eval_exp (QPow e p) m s ->
-        n == m.
-  Proof.
-    move=> e IH p n m s Hn Hm.
-    inversion_clear Hn; inversion_clear Hm.
-    rewrite (eqP (IH _ _ _ H H0)).
-    exact: eqxx.
-  Qed.
-
-  Lemma eval_exp_unique :
-          forall e n m s, eval_exp e n s -> eval_exp e m s -> n == m.
-  Proof.
-    move=> e; elim: e.
-    - exact: eval_qvar_unique.
-    - exact: eval_qconst_unique.
-    - exact: eval_qunop_unique.
-    - exact: eval_qbinop_unique.
-    - exact: eval_qpow_unique.
-  Qed.
-
-  Lemma eval_program_empty :
-    forall (s1 s2 : State.t),
-      eval_program s1 [::] s2 -> s1 = s2.
-  Proof.
-    move=> s1 s2 H; by inversion_clear H.
-  Qed.
+  Fixpoint eval_program (s : State.t) (p : program) : State.t :=
+    match p with
+    | [::] => s
+    | hd::tl => eval_program (eval_instr s hd) tl
+    end.
 
   Lemma eval_program_singleton :
     forall (i : instr) (s1 s2 : State.t),
-      eval_program s1 ([:: i]) s2 ->
-      eval_instr s1 i s2.
+      eval_program s1 ([:: i]) = s2 ->
+      eval_instr s1 i = s2.
   Proof.
-    move=> i s1 s2 H; inversion_clear H.
-    move: (eval_program_empty H1) => {H1} H1.
-    rewrite -H1.
-    exact: H0.
+    move=> i s1 s2 H; assumption.
   Qed.
 
   Lemma eval_program_cons :
     forall (hd : instr) (tl : program) (s1 s2 : State.t),
-      eval_program s1 (hd::tl) s2 ->
+      eval_program s1 (hd::tl) = s2 ->
       exists s3 : State.t,
-        eval_instr s1 hd s3 /\ eval_program s3 tl s2.
+        eval_instr s1 hd = s3 /\ eval_program s3 tl = s2.
   Proof.
     move=> hd tl s1 s2 H.
-    inversion_clear H.
-    exists s3; split; assumption.
+    exists (eval_instr s1 hd); split.
+    - reflexivity.
+    - assumption.
   Qed.
 
   Lemma eval_program_concat :
     forall (p1 p2 : program) (s1 s2 s3 : State.t),
-      eval_program s1 p1 s2 ->
-      eval_program s2 p2 s3 ->
-      eval_program s1 (p1 ++ p2) s3.
+      eval_program s1 p1 = s2 ->
+      eval_program s2 p2 = s3 ->
+      eval_program s1 (p1 ++ p2) = s3.
   Proof.
-    move=> p1; elim: p1.
+    move=> p1; elim: p1 => /=.
     - move=> p2 s1 s2 s3 He1 He2.
-      move: (eval_program_empty He1) => {He1} He1.
-      rewrite He1.
-      exact: He2.
+      by rewrite He1.
     - move=> hd tl H p2 s1 s2 s3 He1 He2.
       move: (eval_program_cons He1) => {He1} [s4 [He1 He4]].
-      apply: (EQCons He1).
-      apply: (H _ _ _ _ He4).
-      exact: He2.
+      move: (H _ _ _ _ He4 He2) => Htlp2.
+      rewrite He1; assumption.
   Qed.
 
   Lemma eval_program_split :
     forall (p1 p2 : program) (s1 s2 : State.t),
-      eval_program s1 (p1 ++ p2) s2 ->
+      eval_program s1 (p1 ++ p2) = s2 ->
       exists s3 : State.t,
-        eval_program s1 p1 s3 /\ eval_program s3 p2 s2.
+        eval_program s1 p1 = s3 /\ eval_program s3 p2 = s2.
   Proof.
     move=> p1; elim: p1.
     - move=> p2 s1 s2 H1.
       exists s1; split.
-      + exact: EQEmpty.
+      + reflexivity.
       + exact: H1.
     - move=> hd tl H p2 s1 s2 He1.
       move: (eval_program_cons He1) => {He1} [s3 [He13 He32]].
       move: (H _ _ _ He32) => {H} [s4 [He34 He42]].
       exists s4; split.
-      + exact: (EQCons He13 He34).
+      + rewrite /= He13.
+        assumption.
       + exact: He42.
   Qed.
 
@@ -487,30 +341,20 @@ Module MakeQhasm (V : SsrOrderedType).
     | QAnd e1 e2 => VS.union (vars_bexp e1) (vars_bexp e2)
     end.
 
-  Inductive eval_bexp : bexp -> bool -> State.t -> Prop :=
-  | EQTrue : forall s, eval_bexp QTrue true s
-  | EQEq :
-      forall e1 e2 n1 n2 s,
-        eval_exp e1 n1 s ->
-        eval_exp e2 n2 s ->
-        eval_bexp (QEq e1 e2) (n1 == n2) s
-  | EQCong :
-      forall e1 e2 n1 n2 p s,
-        eval_exp e1 n1 s ->
-        eval_exp e2 n2 s ->
-        eval_bexp (QCong e1 e2 p) (n1 === n2 # (Zpos p)) s
-  | EQAnd :
-      forall e1 e2 b1 b2 s,
-        eval_bexp e1 b1 s ->
-        eval_bexp e2 b2 s ->
-        eval_bexp (QAnd e1 e2) (b1 && b2) s.
+  Fixpoint eval_bexp (e : bexp) (s : State.t) : Prop :=
+    match e with
+    | QTrue => True
+    | QEq e1 e2 => eval_exp e1 s = eval_exp e2 s
+    | QCong e1 e2 p => modulo (eval_exp e1 s) (eval_exp e2 s) (Zpos p)
+    | QAnd e1 e2 => eval_bexp e1 s /\ eval_bexp e2 s
+    end.
 
   Definition valid (f : bexp) : Prop :=
-    forall s : State.t, eval_bexp f true s.
+    forall s : State.t, eval_bexp f s.
 
   Definition entails (f g : bexp) : Prop :=
     forall s : State.t,
-      eval_bexp f true s -> eval_bexp g true s.
+      eval_bexp f s -> eval_bexp g s.
 
   Record spec : Type :=
     mkSpec { spre : bexp;
@@ -519,9 +363,9 @@ Module MakeQhasm (V : SsrOrderedType).
 
   Definition valid_spec (s : spec) : Prop :=
     forall s1 s2,
-      eval_bexp (spre s) true s1 ->
-      eval_program s1 (sprog s) s2 ->
-      eval_bexp (spost s) true s2.
+      eval_bexp (spre s) s1 ->
+      eval_program s1 (sprog s) = s2 ->
+      eval_bexp (spost s) s2.
 
   Local Notation "s |= f" := (eval_bexp f true s) (at level 74, no associativity).
   Local Notation "f ===> g" := (entails f g) (at level 82, no associativity).
@@ -530,30 +374,9 @@ Module MakeQhasm (V : SsrOrderedType).
   Local Notation "|= s" := (valid_spec s) (at level 83).
 
   Definition counterexample (sp : spec) (s : State.t) : Prop :=
-    eval_bexp (spre sp) true s /\
+    eval_bexp (spre sp) s /\
     exists s' : State.t,
-      eval_program s (sprog sp) s' /\ eval_bexp (spost sp) false s'.
-
-  Lemma eval_bexp_unique :
-    forall e a b s, eval_bexp e a s -> eval_bexp e b s -> a == b.
-  Proof.
-    move=> e; elim: e.
-    - move=> a b s Hea Heb.
-      inversion_clear Hea; inversion_clear Heb.
-      exact: eqxx.
-    - move=> e1 e2 a b s Hea Heb.
-      inversion_clear Hea; inversion_clear Heb.
-      rewrite (eqP (eval_exp_unique H H1)) (eqP (eval_exp_unique H0 H2)).
-      exact: eqxx.
-    - move=> e1 e2 p a b s Hea Heb.
-      inversion_clear Hea; inversion_clear Heb.
-      rewrite (eqP (eval_exp_unique H H1)) (eqP (eval_exp_unique H0 H2)).
-      exact: eqxx.
-    - move=> e1 IH1 e2 IH2 a b s Hea Heb.
-      inversion_clear Hea; inversion_clear Heb.
-      rewrite (eqP (IH1 _ _ _ H H1)) (eqP (IH2 _ _ _ H0 H2)).
-      exact: eqxx.
-  Qed.
+      eval_program s (sprog sp) = s' /\ (~ eval_bexp (spost sp) s').
 
   Lemma spec_empty :
     forall f g,
@@ -561,7 +384,7 @@ Module MakeQhasm (V : SsrOrderedType).
   Proof.
     move=> f g He s Hf.
     apply: (He s _ Hf).
-    apply: EQEmpty.
+    reflexivity.
   Qed.
 
   Lemma spec_strengthing :
@@ -587,12 +410,11 @@ Module MakeQhasm (V : SsrOrderedType).
       |= {{ f }} [::hd] {{ g }} -> |= {{ g }} tl {{ h }} ->
       |= {{ f }} (hd::tl) {{ h }}.
   Proof.
-    move=> f g h hd tl Hhd Htl s1 s2 Hf Hp.
-    inversion_clear Hp.
-    apply: (Htl s3 _ _ H0).
-    apply: (Hhd s1 _ Hf).
-    apply: (EQCons H).
-    exact: EQEmpty.
+    move=> f g h hd tl Hshd Hstl s1 s2 /= Hf Hp.
+    move: (eval_program_cons Hp) => {Hp} [s3 [Hhd Htl]].
+    apply: (Hstl _ _ _ Htl) => /=.
+    apply: (Hshd _ _ _ Hhd) => /=.
+    assumption.
   Qed.
 
   Lemma spec_split_post :
@@ -601,11 +423,35 @@ Module MakeQhasm (V : SsrOrderedType).
       |= {{ f }} p {{ g2 }} ->
       |= {{ f }} p {{ QAnd g1 g2 }}.
   Proof.
-    move=> f g1 g2 p Hg1 Hg2 s1 s2 Hf Hp.
-    move: (Hg1 s1 s2 Hf Hp) => {Hg1} Hg1.
-    move: (Hg2 s1 s2 Hf Hp) => {Hg2} Hg2.
-    exact: (EQAnd Hg1 Hg2).
+    move=> f g1 g2 p Hg1 Hg2 s1 s2 /= Hf Hp.
+    move: (Hg1 s1 s2 Hf Hp) => /= {Hg1} Hg1.
+    move: (Hg2 s1 s2 Hf Hp) => /= {Hg2} Hg2.
+    exact: (conj Hg1 Hg2).
   Qed.
+
+
+
+  (** Well-formed programs *)
+
+  Definition lvals_instr (i : instr) : VS.t :=
+    match i with
+    | QAssign v _ => VS.singleton v
+    | QSplit vh vl _ _ => VS.add vh (VS.singleton vl)
+    end.
+
+  Definition well_formed_instr (vs : VS.t) (i : instr) : bool :=
+    match i with
+    | QAssign v e => VS.subset (vars_exp e) vs
+    | QSplit vh vl e p => VS.subset (vars_exp e) vs
+    end.
+
+  Fixpoint well_formed_program (vs : VS.t) (p : program) : bool :=
+    match p with
+    | [::] => true
+    | hd::tl =>
+      well_formed_instr vs hd &&
+                        well_formed_program (VS.union (lvals_instr hd) vs) tl
+    end.
 
 End MakeQhasm.
 
